

Design and Analysis of algorithms

(11/03/22)

Ans. 1 Asymptotic notations are used in to find the complexity of an algorithm when input is very large.

• Big O(θ): $f(n) = O(g(n))$

iff

$$f(n) \leq Cg(n)$$

$$\forall n \geq n_0$$

for some constant $C > 0$

$g(n)$ is "tight upper bound" of $f(n)$.

• Big Omega (Ω): $f(n) = \Omega(g(n))$

iff

$$f(n) \geq Cg(n)$$

$$\forall n \geq n_0$$

for some constant $C > 0$

$g(n)$ is "tight lower bound" of $f(n)$.

• Big Theta (Θ):

$$f(n) = \Theta(g(n))$$

iff

$$C_1 g(n) \leq f(n) \leq C_2 g(n)$$

$$\forall n \geq \max(n_1, n_2)$$

for some constant $C_1 > 0$ and $C_2 > 0$.

$g(n)$ is both "tight upper bound and lower bound" of $f(n)$.

Ans. 2 for $(i = 1 \text{ to } n) \{ i = i * 2; \}$

1, 2, 4, 8, ... n

let k^{th} term = n

$$n = 1 \cdot (2^{k-1})$$

taking log on both sides

$$\log n = (k-1) \log_2 2$$

$$k = \log n + 1$$

$$O(1 + \log n)$$

$$O(\log n)$$

Ans

Ans. 3 $T(n) = 3T(n-1) - \text{①}$

putting $n=n-1$ in eq. (1)

$$T(n-1) = 3T(n-2) - \text{②}$$

put (2) in (1)

$$T(n) = 9T(n-2)$$

putting $n=n-2$ in eqⁿ (1)

$$T(n-2) = 3T(n-3) - \text{③}$$

$$T(n) = 27T(n-3)$$

$$T(n) = 3^k T(n-k)$$

$$n-k=0$$

$$n=k$$

$$T(n) = 3^n T(n-n)$$

$$= 3^n T(0)$$

$$= 3^n$$

$$O(3^n) \text{ Ans}$$

Ans. 4 $T(n) = 2T(n-1) - \text{①}$

$n=n-1$ in eqⁿ (1)

$$T(n-1) = 2T(n-2) - \text{②}$$

$$T(n) = 4T(n-2) - \text{③}$$

putting, $n=n-2$ in eq. 1

$$T(n-2) = 2T(n-3) - \text{④}$$

$$T(n) = 8T(n-3)$$

$$T(n) = 2^k T(n-k)$$

$$n-k=0$$

$$k=n$$

$$T(n) = 2^n T(n-n)$$

$$= 2^n T(0)$$

$$= 2^n$$

$$O(2^n) = \text{Ans}$$

Ans-5

```
int i=1, s=1;
while (s<=n);
{
    i++; s=s+i;
    printf("#");
}
```

$i = 1 \quad 2 \quad 3 \quad 4 \quad 5 \quad 6 \dots$

$$s = 1 + 3 + 6 + 10 + 15 + \dots + n$$

$$\text{sum of } s = 1 + 3 + 6 + 10 + \dots + n \quad - (1)$$

$$\text{also } s = 1 + 3 + 6 + 10 + \dots + n-1 + n \quad - (2)$$

from (1) - (2)

$$0 = 1 + 2 + 3 + 4 + \dots + n - n$$

$$T_k = 1 + 2 + 3 + 4 + \dots + k$$

$$T_k = \frac{1}{2} k(k+1)$$

for k

$$1 + 2 + 3 + \dots + k \leq n$$

$$k(k+1)/2 \leq n$$

$$(k^2 + k)/2 \leq n$$

$$O(k^2) \leq n$$

$$k = O(\sqrt{n})$$

$$T(n) = O(\sqrt{n})$$

$$O(n^{1/2})$$

Ans \rightarrow

Ans. 6 void function (int n)

{

int i, count = 0;

for (i = 1; i * i ≤ n; i++)

count++;

}

$O(1 + \sqrt{n} + \sqrt{n} + \sqrt{n})$

$O(1 + 3\sqrt{n})$

$O(3\sqrt{n})$

$O(\sqrt{n})$

$O(n^{1/2})$ Ans

Ans. 7 void function (int n)

{

int i, j, k, count = 0;

for (i = n/2; i ≤ n; i++)

for (j = 1; j ≤ n; j = j * 2)

for (k = 1; k ≤ n; k = k * 1)

count++;

}

i j k

$n/2$ 1 1

↓ 2

log n 4

n

→ log n

$O(n/2 \times \log n \times \log n)$

$O(n(\log n)^2)$ Ans

$n/2$

✓

Ans. 8 function (int n)

```

{
    if (n == 1)
        return;
    for (i = 1 to n)
    {
        for (j = 1 to n)
        {
            printf("%x");
        }
    }
    function (n-3);
}

```

n	i	j
n	1	j
		⋮
	2	n
	1	⋮
n-3	n	n
	⋮	⋮
	⋮	⋮
n-6	⋮	⋮
	⋮	⋮

$$1 + 4 + 7 + \dots n$$

$$n = 1 + 3(K-1)$$

$$= 3K - 2$$

$$K = \frac{n+2}{3}$$

✓

no. of terms

$$\frac{n+2}{6} \left[2 + \frac{(n-1) \times 3}{3} \right]$$

$$\left[\frac{n+2}{6} (n+1) \right] n^2$$

$$O \left[\frac{n^2 + 3n + 2}{6} \times n^2 \right]$$

$$O[n^4] \text{ Ans.}$$

Ans. 9

void function(int n)

{

for (i=1 to n) (n)

{

(n)

(n^2)

(n^2)

for (j=1; j <= n; j=j+1)

printf("* "); $j(n^2)$;

}

}

$O(n + n^2 + n^2 + n^2)$

$O(3n^2 + n)$

$O(n^2)$
= $Ans.$